WIP

theories/vir/mcfg_contextual.v
@@ -18,59 +18,100 @@ Section mcfg_contextual.
 
   Context `(sheapGS Σ, checkedoutGS Σ, heapbijGS Σ).
 
+  (* Invariant for frame-related resources across a single function call that
+     is satisfied by the fundamental theorem *)
   Definition frame_inv i_t i_s :=
-    (frame_WF i_t i_s ∗ checkout ∅ ∗ stack_tgt i_t ∗ stack_src i_s)%I.
+    (frame_WF i_t i_s ∗ checkout ∅ ∗ stack_tgt i_t ∗ stack_src i_s ∗
+       ⌜(length i_s > 0)%Z → (length i_t > 0)%Z⌝)%I.
 
   (* An obligation for each of the defined calls; it satisfies the external
       call specifications *)
-  Definition context_rel_call_inv
-      (f : ∀ T : Type, CallE T → L0'expr T)
-      (g : ∀ T : Type, CallE T → L0'expr T) :=
-    (□ (∀ fn1 fn2 dt1 dt2 attr1 attr2 args1 args2 C,
-          let call1 := ExternalCall dt1 fn1 args1 attr1 in
-          let call2 := ExternalCall dt2 fn2 args2 attr2 in
-          call_ev call1 call2 C -∗
-          ⟅ f _ (Call dt1 fn1 args1 attr1) ⟆ ⪯
-          ⟅ g _ (Call dt2 fn2 args2 attr2) ⟆
-          [[ (fun v1 v2 => call_ans call1 v1 call2 v2 C) ⤉ ]]) )%I.
-
-  (* Should follow by reflexivity theorem *)
-  Definition context_rel_refl
-      (f : ∀ T : Type, CallE T → L0'expr T)
-      (g : ∀ T : Type, CallE T → L0'expr T) :=
-    (□ (∀ fn1 fn2 dt attr args1 args2 C,
-          arg_val_rel (fn1, args1) (fn2, args2) C -∗
-          ⟅ f _ (Call dt fn1 args1 attr) ⟆ ⪯
-          ⟅ g _ (Call dt fn2 args2 attr) ⟆
-          [[ (fun x y => res_val_rel x y C) ⤉ ]]))%I.
-
-  (* Definition context_call *)
-  (*     (f : ∀ T : Type, CallE T → L0'expr T) := *)
-  (*   (forall τ addr args attrs, *)
-  (*     f uvalue (Call τ addr args (FNATTR_Internal :: attrs)) = *)
-  (*     f uvalue (Call τ addr args attrs)) /\ *)
-  (*   (forall τ addr args attrs, *)
-  (*     f uvalue (Call τ addr args (FNATTR_External:: attrs)) = *)
-  (*     f uvalue (Call τ addr args attrs)). *)
-
   Definition context_rel
       (f : ∀ T : Type, CallE T → L0'expr T)
       (g : ∀ T : Type, CallE T → L0'expr T) :=
-    (context_rel_call_inv f g ∗ context_rel_refl f g)%I.
+    (□ (∀ fn1 fn2 dt1 dt2 args1 args2 C,
+          let call1 := ExternalCall dt1 fn1 args1 nil in
+          let call2 := ExternalCall dt2 fn2 args2 nil in
+          call_ev call1 call2 C -∗
+          ⟅ f _ (Call dt1 fn1 args1 nil) ⟆ ⪯
+          ⟅ g _ (Call dt2 fn2 args2 nil) ⟆
+          [[ (fun v1 v2 => call_ans call1 v1 call2 v2 C) ⤉ ]]) )%I.
 
-  Theorem Proper_interp_mrec' {R}
-    (f g : ∀ T : Type, LLVMEvents.CallE T → L0'expr T) a1 a2
-    (Ψ : R -d> R -d> iPropI Σ) i_t i_s :
+
+  Notation st_expr_rel' R1 R2 :=
+    (@st_exprO' vir_lang R1 -d> @st_exprO' vir_lang R2 -d> iPropI Σ).
+
+  (* Auxiliary definitions for [Proper_interp_mrec] *)
+  (* Because [sim_expr] includes stateful interpretation, showing properness result
+    for [interp_mrec] amounts to proving a simulation *)
+  Local Definition interp_mrec_pred :=
+    fun (Φ:st_expr_rel' _ _) (e_t:st_expr' vir_lang _) (e_s:st_expr' vir_lang _) =>
+      (∃ f g t dv args attr σ_t σ_s,
+          ⌜e_t = observe (⟦ interp_mrec f (f uvalue (Call t dv args attr)) ⟧ σ_t)⌝ ∗
+          ⌜e_s = observe (⟦ interp_mrec g (g uvalue (Call t dv args attr)) ⟧ σ_s)⌝ ∗
+          context_rel f g ∗
+          sim_coindF Φ
+              (observe (⟦ ⟅ (f uvalue (Call t dv args attr)) ⟆ ⟧ σ_t))
+              (observe (⟦ ⟅ (g uvalue (Call t dv args attr)) ⟆ ⟧ σ_s)))%I.
+
+  Local Definition interp_mrec_rec :=
+    fun (Φ:st_expr_rel' _ _) (e_t:st_expr' vir_lang _) (e_s:st_expr' vir_lang _) =>
+      ((∃ f g t dv args attr σ_t σ_s,
+          ⌜e_t = observe (⟦ interp_mrec f (f uvalue (Call t dv args attr)) ⟧ σ_t)⌝ ∗
+          ⌜e_s = observe (⟦ interp_mrec g (g uvalue (Call t dv args attr)) ⟧ σ_s)⌝ ∗
+         context_rel f g ∗
+         sim_coindF Φ
+          (observe (⟦ ⟅ (f uvalue (Call t dv args attr)) ⟆ ⟧ σ_t))
+          (observe (⟦ ⟅ (g uvalue (Call t dv args attr)) ⟆ ⟧ σ_s)))
+        ∨ sim_coindF Φ e_t e_s)%I.
+
+  Local Instance interp_mrec_pred_ne:
+    NonExpansive (interp_mrec_pred: st_expr_rel' _ _ -d> st_expr_rel' _ _).
+  Proof.
+    intros x y *. solve_proper_prepare. do 18 f_equiv; try solve_proper.
+  Qed.
+
+  Local Instance interp_mrec_rec_ne:
+    NonExpansive (interp_mrec_rec: st_expr_rel' _ _ -d> st_expr_rel' _ _).
+  Proof.
+    intros x y *. solve_proper_prepare. repeat f_equiv; try solve_proper.
+  Qed.
+
+  From Equations Require Import Equations.
+
+  Lemma vir_call_ev_nil i_t i_s t dv args :
+    frame_inv i_t i_s -∗
+    dval_rel dv dv -∗
+    vir_call_ev Σ (ExternalCall t dv args []) (ExternalCall t dv args []) (∅, i_t, i_s).
+  Admitted.
+
+  Theorem Proper_mrec
+    (f g : ∀ T : Type, LLVMEvents.CallE T → L0'expr T)
+    (Ψ : _ -d> _ -d> iPropI Σ) i_t i_s t dv args attr:
+    dval_rel dv dv -∗
     frame_inv i_t i_s -∗
     context_rel f g -∗
-    <pers>
-    (frame_inv i_t i_s -∗ ⟅ a1 ⟆ ⪯ ⟅ a2 ⟆ [[ (fun x y => Ψ x y ∗ frame_inv i_t i_s) ⤉ ]]) -∗
-    interp_mrec f a1 ⪯ interp_mrec g a2
+    mrec f (Call t dv args attr) ⪯ mrec g (Call t dv args attr)
     [[ (fun x y => Ψ x y ∗ frame_inv i_t i_s) ⤉ ]].
   Proof.
-    iIntros "Hinv Hrel #Hr".
-    iSpecialize ("Hr" with "Hinv").
-  Admitted.
+    rewrite /mrec.
+    iIntros "#Hdv Hinv #Hrel"; iIntros (??) "SI".
+
+    iApply (sim_coindF_strong_coind interp_mrec_pred); cycle 1.
+    { rewrite /interp_mrec_pred.
+      iExists f, g, t, dv, args, attr, σ_t, σ_s.
+      do 2 (iSplitL ""; first done); iFrame "Hrel".
+      rewrite /call_ev; cbn -[state_interp].
+      iSpecialize ("Hrel" $! dv dv t t args args (∅, i_t, i_s)).
+      iPoseProof (vir_call_ev_nil with "Hinv Hdv") as "Hev".
+      iSpecialize ("Hrel" with "Hev SI").
+      iMod "Hrel". admit. }
+
+    iModIntro.
+
+  Admitted. (* TODO : Port over proof *)
+
+(* -------------------------------------------------------------------------- *)
 
   (* Type declaration for function definitions, i.e. an association list for
      function definitions with [dvalue] keys. *)
@@ -84,6 +125,8 @@ Section mcfg_contextual.
   Definition fundefs_no_attr (fd : fundefs) :=
     forallb (fun '(_, def) => fundef_no_attr def) fd.
 
+(* -------------------------------------------------------------------------- *)
+
   Lemma sim_external_call dτ addr_t addr_s args_t args_s l i_t i_s:
     frame_WF i_t i_s -∗
     stack_tgt i_t -∗
@@ -93,430 +136,127 @@ Section mcfg_contextual.
     ([∗ list] x;y ∈ args_t;args_s, uval_rel x y) -∗
     ⟅ dargs <- Util.map_monad (λ uv : uvalue, pickUnique uv) args_t;;
     trigger (ExternalCall dτ addr_t (map dvalue_to_uvalue dargs) l) ⟆
-    ⪯
-    ⟅ dargs <- Util.map_monad (λ uv : uvalue, pickUnique uv) args_s;;
+      ⪯
+      ⟅ dargs <- Util.map_monad (λ uv : uvalue, pickUnique uv) args_s;;
     trigger (ExternalCall dτ addr_s (map dvalue_to_uvalue dargs) l) ⟆
-    [[ (fun x y =>
-    uval_rel x y ∗ stack_tgt i_t ∗ stack_src i_s ∗
-    checkout ∅) ⤉ ]].
+      [[ (fun x y =>
+            uval_rel x y ∗ stack_tgt i_t ∗ stack_src i_s ∗
+              checkout ∅) ⤉ ]].
+  Proof. Admitted.
+
+  (* -------------------------------------------------------------------------- *)
+
+  (* Utility TODO: Move *)
+  Lemma dval_rel_lookup_defn_cons {B fn_t fn_s fn_t' fn_s'} e_t e_s F :
+    dval_rel fn_t fn_s -∗
+    dval_rel fn_t' fn_s' -∗
+    ([∗ list] v_t;v_s ∈ F.*1;F.*1, dval_rel v_t v_s) -∗
+
+    (* Both match on the head of the list *)
+    ⌜(lookup_defn fn_t ((fn_t', e_t) :: F) = Some e_t /\
+        lookup_defn fn_s ((fn_s', e_s) :: F) = Some e_s) ∨
+
+    (* Both match on an element in [F] *)
+    (exists f g,
+      lookup_defn fn_t F = Some f /\
+      lookup_defn fn_s F = Some g /\
+      lookup_defn fn_t ((fn_t', e_t) :: F) = Some f /\
+      lookup_defn fn_s ((fn_s', e_s) :: F) = Some g) ∨
+
+    (* Or it is not found *)
+    (lookup_defn fn_t ((fn_t', e_t) :: F) = None /\
+      lookup_defn (B := B) fn_s ((fn_s', e_s) :: F) = None)⌝.
+  Proof.
+    iIntros "Hv Hv' HF"; cbn.
+    destruct (RelDec.rel_dec fn_s fn_s') eqn: Ht;
+      [ iLeft; iSplit; eauto; reldec | iRight ]; reldec.
+    (* Head *)
+    { iDestruct (dval_rel_inj with "Hv Hv'") as "%He"; subst.
+      by rewrite Util.eq_dec_eq. }
+
+    (* Rest *)
+    { iDestruct (dval_rel_ne_inj with "Hv Hv'") as "%He".
+      assert (Hs: fn_s' <> fn_s) by eauto. specialize (He Hs).
+      rewrite Util.eq_dec_neq; eauto.
+
+      destruct (lookup_defn fn_s F) eqn: Hf_t.
+      { iDestruct (dval_rel_lookup_some with "Hv HF") as %Hft.
+        specialize (Hft _ Hf_t); destruct Hft as (?&Hft).
+        iLeft; iPureIntro; eauto.
+        exists x, b; split; [ | split]; eauto. }
+
+      { iDestruct (dval_rel_lookup_none with "Hv HF") as %Hft.
+        specialize (Hft Hf_t).
+        iRight; iPureIntro; eauto. } }
+  Qed.
+
+  Lemma fundef_no_attr_eq def :
+    fundef_no_attr def ->
+    (dc_attrs (df_prototype def)) = nil.
   Proof. Admitted.
 
   (* The contextual refinement on [denote_mcfg]. *)
   Lemma contextual_denote_mcfg :
-    ∀ γ_t γ_s dv dv' e_t e_s main C,
-    fundefs_no_attr C ->
-    fundef_no_attr e_t ->
-    fundef_no_attr e_s ->
-    □ fun_logrel e_t e_s ∅ -∗
-      checkout ∅ -∗
-      stack_tgt [γ_t] -∗
-      stack_src [γ_s] -∗
-      dval_rel dv dv' -∗
-      ([∗ list] v_t;v_s ∈ C.*1;C.*1, dval_rel v_t v_s) -∗
-      denote_mcfg ((dv, e_t) :: C) DTYPE_Void (DVALUE_Addr main) []
-      ⪯
-      denote_mcfg ((dv', e_s) :: C) DTYPE_Void (DVALUE_Addr main) []
-      [[ (λ x y : uvalue, ⌜obs_val x y⌝) ⤉ ]].
+    ∀ γ_t γ_s addr_t addr_s e_t e_s main F,
+      fun_WF e_t ->
+      fun_WF e_s ->
+      fundefs_WF F nil ->
+      fundefs_no_attr F ->
+      fundef_no_attr e_t ->
+      fundef_no_attr e_s ->
+      □ fun_logrel e_t e_s ∅ -∗
+        checkout ∅ -∗
+        stack_tgt [γ_t] -∗
+        stack_src [γ_s] -∗
+        dval_rel addr_t addr_s -∗
+        ([∗ list] v_t;v_s ∈ F.*1;F.*1, dval_rel v_t v_s) -∗
+        denote_mcfg ((addr_t, e_t) :: F) DTYPE_Void (DVALUE_Addr main) []
+        ⪯
+        denote_mcfg ((addr_s, e_s) :: F) DTYPE_Void (DVALUE_Addr main) []
+        [[ (λ x y : uvalue, ⌜obs_val x y⌝) ⤉ ]].
   Proof.
-    iIntros (???????? HC H_t H_s) "#Hfun Hc Hs_t Hs_s #Hdv #Hfun_keys".
-    rewrite /denote_mcfg.
+    iIntros (???????? WF_t WF_s WF_F HC H_t H_s) "#Hfun Hc Hs_t Hs_s #Hdv #Hfun_keys".
 
+    (* The frame invariant holds. *)
     iAssert (frame_inv [γ_t] [γ_s])%I with "[Hc Hs_t Hs_s]" as "Hinv".
     { by iFrame. }
 
     iPoseProof
-      (Proper_interp_mrec' _ _ _ _ (λ x y : uvalue, ⌜obs_val x y⌝)%I [γ_t] [γ_s]
+      (Proper_mrec _ _ (λ x y : uvalue, ⌜obs_val x y⌝)%I [γ_t] [γ_s]
         with "Hinv") as "Hrec"; eauto.
     iApply (sim_expr'_bupd_mono with "[] [Hrec]"); last iApply "Hrec".
+
+    (* Establish postcondition; trivial  *)
     { iIntros (??) "HΨ"; iDestruct "HΨ" as (????) "(%HΨ & HI)".
       iExists _, _; iFrame. done. }
 
-    { rewrite /context_rel.
+    rewrite /context_rel; iModIntro.
 
-      iSplitL ""; cycle 1.
-      {  (* REFL *)
-        iIntros (??).
-        iModIntro.
-        iIntros (?????).
-        destruct C0 as ((?&?)&?).
-        rewrite /arg_val_rel. cbn -[denote_function].
-        iIntros "Hev".
-        iDestruct "Hev" as "(#HWF & HC & Hst & Hss & #Hfn & #Hargs)".
-        subst.
+    (* Preparing proof state *)
+    iIntros (fn_t fn_s dτ_t dτ_s args_t args_s C) "Hev";
+      destruct C as ((?&i_t)&i_s);
+    rewrite /call_ev; cbn -[denote_function lookup_defn]; simp vir_call_ev;
+    iDestruct "Hev" as
+      "(#Hfn &%Hdt & %Hattr& #Hargs & HC & #HWF & Hst & Hss & %Hinterp)"; subst.
 
-        destruct (lookup_defn fn2 ((dv', e_s) :: C)) eqn: Hs; cycle 1.
+    (* Do a case analysis on whether the function is in the list of fundefs.
 
-        (* External call case *)
-        { cbn in Hs. destruct_if; reldec.
-          iDestruct (dval_rel_ne_inj with "Hfn Hdv") as %Hne.
-          assert (dv' <> fn2) by eauto.
-          specialize (Hne H3). cbn -[denote_function].
-          destruct (RelDec.rel_dec fn1 dv) eqn: Hfn1; reldec; try done.
-          iPoseProof (dval_rel_lookup_none with "Hfn Hfun_keys") as "%Hlu".
-          rewrite /lookup_defn.
-          specialize (Hlu Hs); rewrite Hlu.
+      Because the context applied to the expression results in a closed term,
+      the function is always found in the context. *)
 
-          rewrite /call_ev; cbn; simp vir_call_ev.
-          rewrite /lookup_defn in Hs. rewrite Hs.
+    iDestruct (dval_rel_lookup_defn_cons e_t e_s F with "Hfn Hdv Hfun_keys") as %Hlu.
+    destruct Hlu as [ (->&->) | [ Hlu | Hlu ] ]; last admit. (* last case is absurd *)
 
-          iApply (sim_expr'_bupd_mono);
-            last iApply (sim_external_call with "HWF Hst Hss HC Hfn Hargs").
-          iIntros (??) "H'".
-          rewrite /lift_post.
-          iDestruct "H'" as (????) "(#Hv' & HC & Hs_t & Hs_s)".
-          iExists _, _; iFrame.
-          repeat (iSplitL ""; first done).
-          simp vir_call_ans; by iFrame. }
+    (* It is the hole *)
+    { apply fundef_no_attr_eq in H_t, H_s; rewrite H_t H_s.
+      assert (Heq : RelDec.rel_dec (T := list fn_attr) nil nil = true) by admit;
+        rewrite Heq.
+      admit. }
 
-        (* Internal call case *)
-        { rewrite /fundefs_rel_WF.
+    (* It is a function in the context *)
+    { destruct Hlu as (f_t & f_s & Hlu_t & Hlu_s & -> & ->).
+      admit. } (* Should follow trivially. *)
 
-          apply lookup_defn_cons_Some in Hs.
-          destruct Hs.
-          (* It is the [e_s] function (the hole) *)
-          { destruct H2; subst; cbn -[denote_function].
-            iDestruct (dval_rel_inj with "Hdv Hfn") as %Hdef; subst.
-            destruct (RelDec.rel_dec fn1 fn1) eqn: Hf; reldec; subst; last done.
-            destruct (RelDec.rel_dec dv' dv') eqn: Hf'; reldec; subst; last done.
-            subst.
+  Admitted.
 
-            iDestruct "HWF" as %HWF; subst.
-            rewrite /fundef_no_attr in H_t, H_s.
-            assert (attr = nil).
-            { admit. }
-            rewrite H2.
-            destruct (RelDec.rel_dec (dc_attrs (df_prototype d)) []); try done.
-            destruct (RelDec.rel_dec (dc_attrs (df_prototype e_t)) []); try done.
-
-            iSpecialize ("Hfun" $! _ _ _ _ HWF with "Hst Hss Hargs HC").
-            iApply sim_expr'_bupd_mono; last (iApply "Hfun").
-            iIntros (??) "H'".
-            rewrite /lift_post.
-            iDestruct "H'" as (????) "(Hs_t & Hs_s & HC & Hval)".
-            iExists _, _; iFrame. subst; iModIntro.
-            repeat (iSplitL ""; first done).
-            simp vir_call_ans; by iFrame. }
-
-          (* It is a function in the context *)
-          { destruct H2. cbn -[denote_function].
-
-            iDestruct (dval_rel_ne_inj with "Hdv Hfn") as "%Hne"; subst.
-            specialize (Hne H2); subst.
-            destruct (RelDec.rel_dec fn1 dv) eqn: Hf; reldec; subst; first done.
-            destruct (RelDec.rel_dec fn2 dv') eqn: Hf'; reldec; subst; first done.
-            clear H2 Hne Hf.
-            iPoseProof (dval_rel_lookup_some with "Hfn Hfun_keys") as "%Hlu".
-            specialize (Hlu _ H3). destruct Hlu as (?&?).
-            rewrite /lookup_defn in H3.
-            rewrite /lookup_defn; rewrite H2 H3.
-
-            (* Juicing out information from the WF of fundefs *)
-            unfold fundefs_WF in WF_s.
-            apply andb_prop_elim in WF_s.
-            destruct WF_s as (Hlen & Wdup_s).
-            apply andb_prop_elim in Hlen. destruct Hlen as (Hlen & Hfun_wf).
-            apply forallb_True in Hfun_wf.
-            rewrite List.Forall_forall in Hfun_wf.
-            assert (Hr_s := H3).
-            apply lookup_defn_Some_In in H3.
-            (* Function [d] is well-formed. *)
-            specialize (Hfun_wf _ H3); cbn in Hfun_wf.
-
-            (* Using [fundefs_logrel] *)
-            assert (Hlen': (length [γf0] > 0)%Z → (length [γf] > 0)%Z) by auto.
-            rewrite /fundefs_logrel. rewrite /lookup_defn in Hr_s.
-            apply lookup_defn_Some_lookup in Hr_s.
-            destruct Hr_s.
-            (* Juice information out of fundef rel WF *)
-            iDestruct "Hrel" as "(Hrel & Hn)".
-            iSpecialize ("Hrel" $! _ _ _ H6).
-            iDestruct "Hrel" as (???) "(#Hdv' & %Hattr & %Hattr' & %Hft & %Hfs)".
-
-            iDestruct (dval_rel_inj with "Hfn Hdv'") as %Hf; subst.
-
-            iSpecialize ("Hlr" $! _ _ _ _ _ _ H7 H6 Hattr Hattr'
-                          with "Hdv'").
-            iDestruct "HWF" as %HWF.
-            iSpecialize ("Hlr" $! _ _ _ _ HWF with "Hst Hss Hargs HC").
-
-            eapply lookup_defn_Some in H2; eauto;cycle 1.
-            { clear -WF_t.
-
-              unfold fundefs_WF in WF_t.
-              apply andb_prop_elim in WF_t.
-              destruct WF_t as (Hlen & Wdup_t).
-              apply andb_prop_elim in Hlen. destruct Hlen as (Hlen & Hfun_wf).
-              apply forallb_True in Hfun_wf.
-              rewrite List.Forall_forall in Hfun_wf.
-              apply Is_true_true_1 in Wdup_t.
-              by apply NoDup_b_NoDup. }
-            subst.
-
-            iApply sim_expr'_bupd_mono; last iApply "Hlr".
-            iIntros (??) "Hin".
-            iDestruct "Hin" as (????) "(Hst & Hss & HC & Hval)".
-            iExists _, _.
-            repeat (iSplitL ""; first done).
-            simp vir_call_ans; subst; by iFrame. } } }
-
-      { (* CALL INV *)
-        iIntros (??).
-        iModIntro.
-        iIntros (???????).
-        destruct C0 as ((?&?)&?).
-        rewrite /call_ev. cbn -[denote_function].
-        iIntros "Hev". simp vir_call_ev.
-        iDestruct "Hev" as
-          "(#Hfn &%Hdt & %Hattr& #Hargs & HC & #HWF & Hst & Hss & %Hinterp)".
-        subst.
-
-        destruct (lookup_defn fn2 ((dv', e_s) :: r_s))
-          eqn: Hs; cycle 1.
-
-        (* External call case *)
-        { cbn in Hs. destruct_if; reldec.
-          iDestruct (dval_rel_ne_inj with "Hfn Hdv") as %Hne.
-          assert (dv' <> fn2) by eauto.
-          specialize (Hne H3). cbn -[denote_function].
-          destruct (RelDec.rel_dec fn1 dv) eqn: Hfn1; reldec; try done.
-          iPoseProof (dval_rel_lookup_none with "Hfn Hv") as "%Hlu".
-          rewrite /lookup_defn.
-          specialize (Hlu Hs); rewrite Hlu.
-
-          rewrite /call_ev; cbn; simp vir_call_ev.
-          rewrite /lookup_defn in Hs. rewrite Hs.
-
-          specialize (WF_attr _ _ _ _ _ _ _ _ Hinterp); subst.
-
-          iApply (sim_expr'_bupd_mono);
-            last iApply (sim_external_call with "HWF Hst Hss HC Hfn Hargs").
-          iIntros (??) "H'".
-          rewrite /lift_post.
-          iDestruct "H'" as (????) "(#Hv' & HC & Hs_t & Hs_s)".
-          iExists _, _; iFrame.
-          repeat (iSplitL ""; first done).
-          simp vir_call_ans; by iFrame. }
-
-        (* Internal call case *)
-        { rewrite /fundefs_rel_WF.
-
-          apply lookup_defn_cons_Some in Hs.
-          destruct Hs.
-          (* It is the [e_s] function (the hole) *)
-          { destruct H2; subst; cbn -[denote_function].
-            iDestruct (dval_rel_inj with "Hdv Hfn") as %Hdef; subst.
-            destruct (RelDec.rel_dec fn1 fn1) eqn: Hf; reldec; subst; last done.
-            destruct (RelDec.rel_dec dv' dv') eqn: Hf'; reldec; subst; last done.
-            subst.
-
-            iDestruct "HWF" as %HWF; subst.
-            iDestruct ("Hf" $! _ _ _) as "(_ & Hf')".
-            specialize (WF_attr _ _ _ _ _ _ _ _ Hinterp); subst.
-
-            iSpecialize ("Hf'" $! _ _ _ _ HWF with "Hst Hss Hargs HC").
-            iApply sim_expr'_bupd_mono; last (iApply "Hf'").
-            iIntros (??) "H'".
-            rewrite /lift_post.
-            iDestruct "H'" as (????) "(Hs_t & Hs_s & HC & Hval)".
-            iExists _, _; iFrame. subst; iModIntro.
-            repeat (iSplitL ""; first done).
-            simp vir_call_ans; by iFrame. }
-
-          (* It is a function in the context *)
-          { destruct H2. cbn -[denote_function].
-
-            iDestruct (dval_rel_ne_inj with "Hdv Hfn") as "%Hne"; subst.
-            specialize (Hne H2); subst.
-            destruct (RelDec.rel_dec fn1 dv) eqn: Hf; reldec; subst; first done.
-            destruct (RelDec.rel_dec fn2 dv') eqn: Hf'; reldec; subst; first done.
-            clear H2 Hne Hf.
-            iPoseProof (dval_rel_lookup_some with "Hfn Hv") as "%Hlu".
-            specialize (Hlu _ H3). destruct Hlu as (?&?).
-            rewrite /lookup_defn in H3.
-            rewrite /lookup_defn; rewrite H2 H3.
-
-            (* Juicing out information from the WF of fundefs *)
-            unfold fundefs_WF in WF_s.
-            apply andb_prop_elim in WF_s.
-            destruct WF_s as (Hlen & Wdup_s).
-            apply andb_prop_elim in Hlen. destruct Hlen as (Hlen & Hfun_wf).
-            apply forallb_True in Hfun_wf.
-            rewrite List.Forall_forall in Hfun_wf.
-            assert (Hr_s := H3).
-            apply lookup_defn_Some_In in H3.
-            (* Function [d] is well-formed. *)
-            specialize (Hfun_wf _ H3); cbn in Hfun_wf.
-
-            (* Using [fundefs_logrel] *)
-            assert (Hlen': (length [γf0] > 0)%Z → (length [γf] > 0)%Z) by auto.
-            rewrite /fundefs_logrel. rewrite /lookup_defn in Hr_s.
-            apply lookup_defn_Some_lookup in Hr_s.
-            destruct Hr_s.
-            (* Juice information out of fundef rel WF *)
-            iDestruct "Hrel" as "(Hrel & Hn)".
-            iSpecialize ("Hrel" $! _ _ _ H6).
-            iDestruct "Hrel" as (???) "(#Hdv' & %Hattr & %Hattr' & %Hft & %Hfs)".
-
-            iDestruct (dval_rel_inj with "Hfn Hdv'") as %Hf; subst.
-
-            specialize (WF_attr _ _ _ _ _ _ _ _ Hinterp); subst.
-            iSpecialize ("Hlr" $! _ _ _ _ _ _ H7 H6 Hattr Hattr'
-                          with "Hdv'").
-            iDestruct "HWF" as %HWF.
-            iSpecialize ("Hlr" $! _ _ _ _ HWF with "Hst Hss Hargs HC").
-
-            eapply lookup_defn_Some in H2; eauto;cycle 1.
-            { clear -WF_t.
-
-              unfold fundefs_WF in WF_t.
-              apply andb_prop_elim in WF_t.
-              destruct WF_t as (Hlen & Wdup_t).
-              apply andb_prop_elim in Hlen. destruct Hlen as (Hlen & Hfun_wf).
-              apply forallb_True in Hfun_wf.
-              rewrite List.Forall_forall in Hfun_wf.
-              apply Is_true_true_1 in Wdup_t.
-              by apply NoDup_b_NoDup. }
-            subst.
-
-            iApply sim_expr'_bupd_mono; last iApply "Hlr".
-            iIntros (??) "Hin".
-            iDestruct "Hin" as (????) "(Hst & Hss & HC & Hval)".
-            iExists _, _.
-            repeat (iSplitL ""; first done).
-            simp vir_call_ans; subst; by iFrame. } } } }
-
-    (* Other obligation that "feels like a duplicate obligation",
-    but is a separate one coming from the body of the [mrec] *)
-    { iModIntro. iIntros "(#HWF & HC & Hst & Hss)".
-
-      iAssert (dval_rel (DVALUE_Addr main) (DVALUE_Addr main))%I as "#Hmain".
-      { rewrite (dval_rel_unfold (DVALUE_Addr _)).
-        cbn. iSplitL ""; try done.
-        iDestruct "Haddr_main" as "(Haddr_main & _)"; done. }
-
-      destruct (lookup_defn (DVALUE_Addr main) ((dv', e_s) :: r_s))
-        eqn: Hs; cycle 1.
-
-      (* External call case *)
-      { cbn in Hs. destruct_if; reldec.
-        iDestruct (dval_rel_ne_inj with "Hmain Hdv") as %Hne.
-        assert (dv' <> DVALUE_Addr main) by eauto.
-        specialize (Hne H3). cbn -[denote_function map_monad].
-        destruct (RelDec.rel_dec (DVALUE_Addr main) dv) eqn: Hfn1;
-          reldec; try done.
-        iPoseProof (dval_rel_lookup_none with "Hmain Hv") as "%Hlu".
-        rewrite /lookup_defn.
-        specialize (Hlu Hs); rewrite Hlu.
-
-        iApply (sim_expr'_bupd_mono);
-          last iApply (sim_external_call with "HWF Hst Hss HC Hmain"); try done.
-        iIntros (??) "H'".
-        rewrite /lift_post.
-        iDestruct "H'" as (????) "(#Hv' & HC & Hs_t & Hs_s)".
-        iExists _, _; iFrame.
-        repeat (iSplitL ""; first done).
-        (iSplitR ""; last done).
-
-        iApply (uval_rel_implies_obs_val with "Hv'"). }
-
-      (* Internal call case *)
-      { apply lookup_defn_cons_Some in Hs.
-        destruct Hs.
-        (* It is the [e_s] function (the hole) *)
-        { destruct H2; inv H2; subst. cbn -[denote_function].
-          iDestruct (dval_rel_inj with "Hdv Hmain") as %Hdef; subst.
-          destruct (RelDec.rel_dec (DVALUE_Addr main) (DVALUE_Addr main))
-            eqn: Hf; reldec; subst; last done.
-          rewrite /fun_logrel.
-          iDestruct "HWF" as %HWF.
-          iDestruct ("Hf" $! _ _ _) as "(_ & Hf')".
-
-          iSpecialize ("Hf'" $! _ _ nil nil HWF with "Hst Hss").
-          cbn -[denote_function].
-          iSpecialize ("Hf'" $! Logic.I with "HC").
-
-          iApply sim_expr'_bupd_mono; last (iApply "Hf'").
-          iIntros (??) "H'".
-          rewrite /lift_post.
-          iDestruct "H'" as (????) "(Hs_t & Hs_s & HC & Hval)".
-          iExists _, _; iFrame. subst; iModIntro.
-          repeat (iSplitL ""; first done).
-          (iSplitR ""; last done).
-          iApply (uval_rel_implies_obs_val with "Hval"). }
-
-        (* It is a function in the context *)
-        { destruct H2; cbn -[denote_function].
-
-          iDestruct (dval_rel_ne_inj with "Hdv Hmain") as "%Hne"; subst.
-          specialize (Hne H2); subst.
-          destruct (RelDec.rel_dec (DVALUE_Addr main) dv) eqn: Hf;
-            reldec; subst; first done.
-          clear H2 Hne Hf.
-          iPoseProof (dval_rel_lookup_some with "Hmain Hv") as "%Hlu".
-          specialize (Hlu _ H3). destruct Hlu as (?&?).
-          rewrite /lookup_defn H2.
-
-          (* Juicing out information from the WF of fundefs *)
-          unfold fundefs_WF in WF_s.
-          apply andb_prop_elim in WF_s.
-          destruct WF_s as (Hlen & Wdup_s).
-          apply andb_prop_elim in Hlen. destruct Hlen as (Hlen & Hfun_wf).
-          apply forallb_True in Hfun_wf.
-          rewrite List.Forall_forall in Hfun_wf.
-          assert (Hr_s := H3).
-          apply lookup_defn_Some_In in H3.
-          (* Function [d] is well-formed. *)
-          specialize (Hfun_wf _ H3); cbn in Hfun_wf.
-
-          (* Using [fundefs_logrel] *)
-          assert (Hlen': (length [γf0] > 0)%Z → (length [γf] > 0)%Z) by auto.
-          rewrite /fundefs_logrel.
-          apply lookup_defn_Some_lookup in Hr_s.
-          destruct Hr_s.
-          (* Juice information out of fundef rel WF *)
-          iDestruct "Hrel" as "(Hrel & Hn)".
-          iSpecialize ("Hrel" $! _ _ _ H6).
-          iDestruct "Hrel" as (???)
-                                "(#Hdv' & %Hattr & %Hattr' & %Hft & %Hfs)".
-
-          iSpecialize ("Hlr" $! _ _ _ _ _ _ H7 H6 Hattr Hattr'
-                        with "Hdv'").
-          iSpecialize ("Hlr" $! _ _ nil nil Hlen' with "Hst Hss").
-          cbn -[denote_function].
-          iSpecialize ("Hlr" $! Logic.I with "HC").
-
-          iDestruct (dval_rel_inj with "Hmain Hdv'") as %Hf; subst.
-
-          eapply lookup_defn_Some in H2; eauto;cycle 1.
-          { clear -WF_t.
-
-            unfold fundefs_WF in WF_t.
-            apply andb_prop_elim in WF_t.
-            destruct WF_t as (Hlen & Wdup_t).
-            apply andb_prop_elim in Hlen. destruct Hlen as (Hlen & Hfun_wf).
-            apply forallb_True in Hfun_wf.
-            rewrite List.Forall_forall in Hfun_wf.
-            apply Is_true_true_1 in Wdup_t.
-            by apply NoDup_b_NoDup. }
-          eauto.
-          subst.
-
-          iApply sim_expr'_bupd_mono; last iApply "Hlr".
-          iIntros (??) "Hin".
-          iDestruct "Hin" as (????) "(Hst & Hss & HC & Hval)".
-          iExists _, _; subst.
-          repeat (iSplitL ""; first done); iFrame.
-          (iSplitR ""; last done).
-
-          iApply (uval_rel_implies_obs_val with "Hval"). } } }
-      Unshelve.
-      all : eauto. all: do 2 constructor.
-    Qed.
-
-
-      { cbn.
-
-
-    Admitted.
-
-  End mcfg_contextual.
+End mcfg_contextual.
